providers/quic/Spec.QUIC.fsti
@@ -69,13 +69,6 @@ val parse_varint: b:bytes{S.length b > 0} -> option (n:nat{n < pow2 62} * vlsize
 
 val lemma_varint: (n:nat62) -> (suff:bytes) -> Lemma (parse_varint S.(encode_varint n @| suff) == Some (n, vlen n,suff))
 
-val lemma_varint_safe : (b1:bytes) -> (b2:bytes) -> Lemma
-  (requires
-    S.length b1 <> 0 /\
-    S.length b2 <> 0 /\
-    parse_varint b1 = parse_varint b2)
-  (ensures parse_varint b1 = None \/ b1 = b2)
-
 
 let max_plain_length : n:nat{forall a. n <= AEAD.max_length a} = pow2 32 - 17
 
